refactor: privatize `is*Instance`

Nerodia/Data/PyNone/Basic.lean
@@ -10,7 +10,8 @@ meta import Nerodia.Internal.ViewMethod
 
 namespace Nerodia
 
-@[inline, irreducible, expose] public def TypeExpr.none : TypeExpr :=
+@[inline, irreducible, expose] -- for Nerodia compiler reduction
+public def TypeExpr.none : TypeExpr :=
   ⟨"None"⟩
 
 public instance : CoeDep (Option α) none TypeExpr := ⟨.none⟩
@@ -28,12 +29,12 @@ public def Typing.none : Typing :=
 public instance : CoeDep (Option α) none Typing := ⟨.none⟩
 public instance : ToTypeExpr none := ⟨none⟩
 
-theorem PyEnvironment.noneRaw_hasType_none {env} : noneRaw env ⦂ none := by
+theorem PyEnvironment.noneRaw_hasType {env} : noneRaw env ⦂ none := by
   simp [PyEnvironment.noneRaw, Typing.none]
 
 open PyEnvironment in
 public instance : NonemptyPy none :=
-  .intro (noneRaw Classical.ofNonempty) noneRaw_hasType_none
+  .intro (noneRaw Classical.ofNonempty) noneRaw_hasType
 
 /-- A Python {lit}`None` constant. -/
 public abbrev PyNone := PyObjectView <| Py none
@@ -42,14 +43,15 @@ open Classical in
 /-- Equivalent to the Python {lit}`self is None`. -/
 @[extern "nerodia_py_object_is_none", view_method]
 public def PyObject.isNone (self : PyObject) : Bool :=
-  @decide (self.raw ⦂ none) (Classical.propDecidable _)
+  self ⦂ none
 
 @[grind _=_]
-public theorem PyObject.isNone_iff_hasType : isNone o ↔ o.raw ⦂ none := by
+public theorem PyObject.isNone_iff_hasType : isNone o ↔ o ⦂ none := by
   simp [PyObject.isNone]
 
-public instance : DecidablePy none :=
-  Internal.decPy (·.isNone) (·.isNone_iff_hasType)
+open PyObject in
+public instance : DecidablePy none := private_decl%
+  (Internal.decPy isNone fun _ => isNone_iff_hasType)
 
 @[simp] public theorem PyNone.isNone_eq_true : (o : PyNone).isNone = true := by
   simp [PyObject.isNone_iff_hasType]
@@ -57,7 +59,7 @@ public instance : DecidablePy none :=
 /-- Returns a reference to the {lit}`None` constant. -/
 @[extern "nerodia_py_environment_none"]
 public def PyEnvironment.none (env : @& PyEnvironment) : PyNone :=
-  ⟨env.noneRaw, noneRaw_hasType_none⟩
+  ⟨env.noneRaw, noneRaw_hasType⟩
 
 /-- Returns the {lit}`None` constant of the Python environment. -/
 @[extern "nerodia_get_py_none"]
